pulse/lib/pulse/lib/Pulse.Lib.ConditionVarWithCodes.fst
@@ -751,7 +751,7 @@ ghost
 fn split #c (b:cvar_t c) (#q #r:slprop) (cq:codeable c q) (cr:codeable c r)
 requires recv b (q ** r)
 ensures recv b q ** recv b r
-opens (add_inv emp_inames b.i)
+opens [b.i]
 {
   unfold recv;
   with p i code. _;
